refactor: make framework DFA parametrized by CFG

Flow/Analysis/Generic.lean
@@ -3,57 +3,57 @@ import Flow.Analysis.CFG
 
 namespace Flow.Analysis.Generic
 
-variable {Node Edge State : Type} [DecidableEq Node] [DecidableEq Edge]
+variable (Node Edge State : Type)
+variable [DecidableEq Node] [DecidableEq Edge]
 
-structure DFA (Node Edge : Type) [DecidableEq Node] [DecidableEq Edge] where
+/-- Generic wrapper for semantics over the CFG.
+    * `ValidCFG` : Links an abstract CFG to the language's concrete invariants.
+    * `LStep`    : proper transition relation (requires ValidCFG)
+    * `LStutter` : silent transition relation (requires ValidCFG)
+-/
+class LangSem where
+  ValidCFG : AnalysisCFG Node Edge -> Type
+  LStep (g : AnalysisCFG Node Edge) (hvalid : ValidCFG g) : EdgeOf g -> State -> State -> Prop
+  LStutter (g : AnalysisCFG Node Edge) (hvalid : ValidCFG g) : Node -> State -> State -> Prop
+
+structure DFA [ls : LangSem Node Edge State] where
   L : Type
   nodeTransfer : Node -> L -> L
   edgeTransfer : Edge -> L -> L
   entry        : L
 
-def DFA.transferAlong
-    (A : DFA Node Edge) (g : AnalysisCFG Node Edge)
-    (e : Edge) (ℓ : A.L) : A.L :=
+variable {Node Edge State : Type}
+variable [DecidableEq Node] [DecidableEq Edge]
+variable [ls : LangSem Node Edge State]
+variable (g : AnalysisCFG Node Edge) (gValid : ls.ValidCFG g)
+
+def DFA.transferAlong (A : DFA Node Edge State) (e : EdgeOf g) (ℓ : A.L) : A.L :=
   A.edgeTransfer e (A.nodeTransfer (g.srcOf e) ℓ)
 
-/-- Generic wrapper for semantics over the CFG.
-    * `LStep` : proper transition relation
-    * `LStutter` : silent transition relation
--/
-class LangSem (Node Edge State : Type)
-    [DecidableEq Node] [DecidableEq Edge] where
-  LStep (g : AnalysisCFG Node Edge) : EdgeOf g -> State -> State -> Prop
-  LStutter : AnalysisCFG Node Edge -> Node -> State -> State -> Prop
-
 /-- RTC of `LStep` along stutter edges. -/
-inductive LSteps [LangSem Node Edge State] (g : AnalysisCFG Node Edge) :
-    Node -> State -> Node -> State -> Prop where
-  | refl  (n : Node) (σ : State) : LSteps g n σ n σ
+inductive LSteps : Node -> State -> Node -> State -> Prop where
+  | refl  (n : Node) (σ : State) : LSteps n σ n σ
   | step  {e : EdgeOf g} {n n'' : Node} {σ σ' σ'' : State} :
-      LangSem.LStep g e σ σ' ->
-      LSteps g (g.dstOf e) σ' n'' σ'' ->
+      LangSem.LStep g gValid e σ σ' ->
+      LSteps (g.dstOf e) σ' n'' σ'' ->
       g.srcOf e = n ->
-      LSteps g n σ n'' σ''
+      LSteps n σ n'' σ''
   | stut  {n n' : Node} {σ σ' σ'' : State} :
-      LangSem.LStutter g n σ σ' ->
-      LSteps g n σ' n' σ'' ->
-      LSteps g n σ n' σ''
+      LangSem.LStutter g gValid n σ σ' ->
+      LSteps n σ' n' σ'' ->
+      LSteps n σ n' σ''
 
 namespace LSteps
 
-variable [LangSem Node Edge State]
-
 /-- lift a single `LStep` to a `LSteps`. -/
-theorem single {g : AnalysisCFG Node Edge} {e : EdgeOf g}
-    {σ σ' : State} (hstep : LangSem.LStep g e σ σ') :
-    LSteps g (g.srcOf e) σ (g.dstOf e) σ' :=
+theorem single {e : EdgeOf g} {σ σ' : State} (hstep : LangSem.LStep g gValid e σ σ') :
+    LSteps g gValid (g.srcOf e) σ (g.dstOf e) σ' :=
   .step hstep (.refl _ _) rfl
 
 /-- transitivity of `LSteps` -/
-theorem trans {g : AnalysisCFG Node Edge}
-    {n n₁ n' : Node} {σ σ₁ σ' : State}
-    (hl : LSteps g n σ n₁ σ₁) (hr : LSteps g n₁ σ₁ n' σ') :
-    LSteps g n σ n' σ' := by
+theorem trans {n n₁ n' : Node} {σ σ₁ σ' : State}
+    (hl : LSteps g gValid n σ n₁ σ₁) (hr : LSteps g gValid n₁ σ₁ n' σ') :
+    LSteps g gValid n σ n' σ' := by
   induction hl with
   | refl _ _ => exact hr
   | step hstep _ hsrc ih => exact .step hstep (ih hr) hsrc
@@ -61,93 +61,75 @@ theorem trans {g : AnalysisCFG Node Edge}
 
 end LSteps
 
-structure DFASemantics [LangSem Node Edge State] (A : DFA Node Edge) where
+/-- Logical semantics linking the DFA to the abstract LangSem relation -/
+structure DFASemantics (A : DFA Node Edge State) where
   Corr : A.L -> State -> Prop
   isInit : State -> Prop
   preserve_entry :
     ∀ {σ : State}, isInit σ -> Corr A.entry σ
   preserve_step :
-    ∀ {g : AnalysisCFG Node Edge} {e : EdgeOf g} {σ σ' : State} {ℓ : A.L},
-      LangSem.LStep g e σ σ' -> Corr ℓ σ -> Corr (A.transferAlong g e ℓ) σ'
+    ∀ {e : EdgeOf g} {σ σ' : State} {ℓ : A.L},
+      LangSem.LStep g gValid e σ σ' -> Corr ℓ σ -> Corr (A.transferAlong g e ℓ) σ'
   preserve_stutter :
-    ∀ {g : AnalysisCFG Node Edge} {n : Node} {σ σ' : State} {ℓ : A.L},
-      LangSem.LStutter g n σ σ' -> Corr ℓ σ -> Corr ℓ σ'
+    ∀ {n : Node} {σ σ' : State} {ℓ : A.L},
+      LangSem.LStutter g gValid n σ σ' -> Corr ℓ σ -> Corr ℓ σ'
 
 /-- a node-indexed labelling is a post-fixpoint of `A`'s transfer if,
     for every `e`, the fact at `srcOf e` after transfer is absorbed
     by the fact at `dstOf e`. -/
-def PostFixpoint
-    (A : DFA Node Edge)
-    (g : AnalysisCFG Node Edge) (rd : Node -> A.L)
-    [Max A.L] : Prop :=
-  ∀ e ∈ g.edges, (A.transferAlong g e (rd (g.srcOf e))) ⊑ (rd (g.dstOf e))
+def PostFixpoint (A : DFA Node Edge State) (rd : Node -> A.L) [Max A.L] : Prop :=
+  ∀ e : EdgeOf g,
+    (A.transferAlong g e (rd (g.srcOf e))) ⊑ (rd (g.dstOf e))
 
-/-- step preservation of analysis correctness: if state `σ`
-    * is abstracted by the result at node `srcOf e`
-    * steps to state `σ'` through `e`
-    then `σ'` is abstracted by the result at node `dstOf e` -/
+/-- step preservation of analysis correctness -/
 theorem step_preserves_corr
-    [LangSem Node Edge State]
-    {A : DFA Node Edge} (S : DFASemantics A)
-    [Max A.L]
-    (mono_absorb :
-      ∀ {ℓ ℓ' : A.L} {σ : State},
-        ℓ ⊑ ℓ' -> S.Corr ℓ σ -> S.Corr ℓ' σ)
-    {g : AnalysisCFG Node Edge} {rd : Node -> A.L}
-    (hpf : PostFixpoint A g rd)
+    {A : DFA Node Edge State} (S : DFASemantics g gValid A) [Max A.L]
+    (mono_absorb : ∀ {ℓ ℓ' : A.L} {σ : State}, ℓ ⊑ ℓ' -> S.Corr ℓ σ -> S.Corr ℓ' σ)
+    {rd : Node -> A.L} (hpf : PostFixpoint g A rd)
     {e : EdgeOf g} {σ σ' : State}
-    (hstep : LangSem.LStep g e σ σ')
+    (hstep : LangSem.LStep g gValid e σ σ')
     (hcorr : S.Corr (rd (g.srcOf e)) σ) :
     S.Corr (rd (g.dstOf e)) σ' :=
-  mono_absorb (hpf e.val e.prop) (S.preserve_step hstep hcorr)
+  mono_absorb (hpf e) (S.preserve_step hstep hcorr)
 
 /-- lift of step preservation through the multi-step closure of the step relation. -/
 theorem steps_preserves_corr
-    [LangSem Node Edge State]
-    {A : DFA Node Edge} (S : DFASemantics A)
-    [Max A.L]
-    (mono_absorb : ∀ {ℓ ℓ' : A.L} {σ : State},
-        ℓ ⊑ ℓ' -> S.Corr ℓ σ -> S.Corr ℓ' σ)
-    {g : AnalysisCFG Node Edge} {rd : Node -> A.L}
-    (hpf : PostFixpoint A g rd)
+    {A : DFA Node Edge State} (S : DFASemantics g gValid A) [Max A.L]
+    (mono_absorb : ∀ {ℓ ℓ' : A.L} {σ : State}, ℓ ⊑ ℓ' -> S.Corr ℓ σ -> S.Corr ℓ' σ)
+    {rd : Node -> A.L} (hpf : PostFixpoint g A rd)
     {n n' : Node} {σ σ' : State}
-    (hsteps : LSteps g n σ n' σ')
+    (hsteps : LSteps g gValid n σ n' σ')
+    -- (hn_mem : n ∈ g.nodes)
     (hcorr : S.Corr (rd n) σ) :
     S.Corr (rd n') σ' := by
   induction hsteps with
   | refl _ _ => exact hcorr
-  | @step e n n'' σ σ' σ'' hstep _ hsrc ih =>
+  | @step e n_src n'' σ_src σ' σ'' hstep _ hsrc ih =>
     apply ih
     simpa [hsrc, hcorr] using
-      (step_preserves_corr S mono_absorb hpf hstep)
+      (step_preserves_corr g gValid S mono_absorb hpf hstep)
   | stut hstut _ ih =>
     exact ih (S.preserve_stutter hstut hcorr)
 
 /-- State `σ` is `Reachable` if there's an initial state `σ₀` such that a
     chain of steps exists from `σ₀` to `σ`. -/
-def Reachable [LangSem Node Edge State] (g : AnalysisCFG Node Edge)
-    (n : Node) (σ : State) (isInit : State -> Prop) : Prop :=
-  ∃ σ₀ : State, isInit σ₀ ∧ LSteps g g.entry σ₀ n σ
+def Reachable (n : Node) (σ : State) (isInit : State -> Prop) : Prop :=
+  ∃ σ₀ : State, isInit σ₀ ∧ LSteps g gValid g.entry σ₀ n σ
 
 /-- If state σ' is `Reachable`, then the analysis result at the node
     corresponding to it is correct.
     Direct application of `steps_preserves_corr` -/
 theorem reachable_corr
-    [LangSem Node Edge State]
-    {A : DFA Node Edge} (S : DFASemantics A)
-    [Max A.L]
-    (mono_absorb :
-      ∀ {ℓ ℓ' : A.L} {σ : State},
-        ℓ ⊑ ℓ' -> S.Corr ℓ σ -> S.Corr ℓ' σ)
-    {g : AnalysisCFG Node Edge} {rd : Node -> A.L}
-    (hpf : PostFixpoint A g rd)
+    {A : DFA Node Edge State} (S : DFASemantics g gValid A) [Max A.L]
+    (mono_absorb : ∀ {ℓ ℓ' : A.L} {σ : State}, ℓ ⊑ ℓ' -> S.Corr ℓ σ -> S.Corr ℓ' σ)
+    {rd : Node -> A.L} (hpf : PostFixpoint g A rd)
     (hentry : A.entry ⊑ (rd g.entry))
     {n : Node} {σ : State}
-    (hreach : Reachable g n σ S.isInit) :
+    (hreach : Reachable g gValid n σ S.isInit) :
     S.Corr (rd n) σ := by
   obtain ⟨σ₀, hinit, hsteps⟩ := hreach
   have h_entry : S.Corr A.entry σ₀ := S.preserve_entry hinit
   have h_rd0   : S.Corr (rd g.entry) σ₀ := mono_absorb hentry h_entry
-  exact steps_preserves_corr S mono_absorb hpf hsteps h_rd0
+  exact steps_preserves_corr g gValid S mono_absorb hpf hsteps h_rd0
 
 end Flow.Analysis.Generic
